bedrock2/src/bedrock2Examples/stackalloc.v
@@ -1,11 +1,7 @@
-Require Import bedrock2.BasicCSyntax bedrock2.NotationsCustomEntry.
+Require Import bedrock2.Syntax bedrock2.NotationsCustomEntry.
 
-Import Syntax BinInt String List.ListNotations.
+Import Syntax.Coercions BinInt String List.ListNotations.
 Local Open Scope string_scope. Local Open Scope Z_scope. Local Open Scope list_scope.
-Local Coercion var (x : string) : Syntax.expr := Syntax.expr.var x.
-Local Definition bedrock_func : Type := String.string * (list String.string * list String.string * cmd).
-Local Coercion name_of_func (f : bedrock_func) := fst f.
-Local Coercion expr.literal : Z >-> expr.
 
 Definition stacktrivial : bedrock_func := let t := "t" in
   ("stacktrivial", ([]:list String.string, [], bedrock_func_body:(stackalloc 4 as t { /*skip*/ }))).
@@ -90,7 +86,7 @@ Section WithParameters.
   From bedrock2 Require Import ToCString Bytedump.
   Local Open Scope bytedump_scope.
   Goal True.
-    let c_code := eval cbv in (byte_list_of_string (@c_module to_c_parameters (stacknondet::nil))) in
+    let c_code := eval cbv in (byte_list_of_string (c_module (stacknondet::nil))) in
     idtac c_code.
   Abort.
 End WithParameters.
